proof/amd64/ref/Keccak1600_ref.ec
@@ -1,12 +1,114 @@
+(******************************************************************************
+   Keccak1600_avx2.ec:
+
+   Correctness proof for the Keccak REF implementation
+
+
+
+******************************************************************************)
+
 require import List Real Int IntDiv CoreMap.
+require BitEncoding.
+import BitEncoding.BitChunking.
 
 from Jasmin require import JModel.
 
+from CryptoSpecs require import JWordList.
 from CryptoSpecs require export Keccakf1600_Spec Keccak1600_Spec.
 from CryptoSpecs require import Bindings.
 
 from JazzEC require import Jazz_ref.
-from JazzEC require import Array5 Array24.
+from JazzEC require import WArray200.
+from JazzEC require import Array25.
+
+(******************************************************************************
+   
+******************************************************************************)
+
+(* MOVE TO CryptoSpecs *)
+op fillstate_at (st: W64.t Array25.t) (at:int) (l: W8.t list) =
+ stwords
+  (WArray200.fill 
+   (fun i => l.[i-at]) at (size l) (stbytes st)).
+
+op addstate_at (st: W64.t Array25.t) (at:int) (l: W8.t list) =
+ stwords
+  (WArray200.fill 
+   (fun i => (stbytes st).[i] `^` l.[i-at]) at (size l) (stbytes st)).
+
+op absorb_spec_ref (r8: int) (tb: int) (l: W8.t list) st =
+ st = ABSORB1600 (W8.of_int tb) r8 l.
+
+op pabsorb_spec_ref r8 l st: bool =
+ 0 < r8 <= 200 /\
+ st = addstate (stateabsorb_iblocks (chunk r8 l) st0) (bytes2state (chunkremains r8 l)).
+
+lemma pabsorb_spec_ref_nil r8:
+ 0 < r8 <= 200 =>
+ pabsorb_spec_ref r8 [] st0.
+proof.
+move=> Hr; rewrite /pabsorb_spec_ref => />.
+rewrite chunk0 /= 1:/#.
+rewrite /stateabsorb_iblocks /= /chunkremains /=.
+admit (* should we add lemmas to the spec? *).
+qed.
 
 
+(******************************************************************************
+   
+******************************************************************************)
+
+lemma state_init_ref_ll:
+ islossless M.__state_init_ref.
+proof.
+proc.
+while true (25-to_uint i).
+ move=> z; auto => /> &m; rewrite ultE of_uintK /= => Hi.
+ by rewrite to_uintD_small /#.
+by auto => /> i Hi; rewrite ultE of_uintK /#.
+qed.
+
+hoare state_init_ref_h _r8:
+ M.__state_init_ref
+ : 0 < _r8 <= 200
+ ==> pabsorb_spec_ref _r8 [] res.
+proof.
+proc.
+conseq (:_ ==> st=st0) => //=.
+ by move=> ? st ->; apply (pabsorb_spec_ref_nil _r8).
+while (0 <= to_uint i <= 25 /\ forall k, 0 <= k < to_uint i => st.[k] = z64).
+ auto => /> &m Hi1 _ IH; rewrite ultE of_uintK /= => Hi2.
+ rewrite to_uintD_small 1:/# /=; split; first smt().
+ by move => k Hk1 Hk2; case: (k=to_uint i{m}) => C; rewrite get_setE /#.
+auto => /> &m Hr1 Hr2; split; first smt().
+move=> i st; rewrite ultE of_uintK /= => ???; have->: to_uint i=25 by smt().
+move=> H; rewrite tP /st0 => j Hj.
+by rewrite createiE 1:// H.
+qed.
+
+phoare state_init_ref_ph _r8:
+ [ M.__state_init_ref
+ : 0 < _r8 <= 200
+ ==> pabsorb_spec_ref _r8 [] res
+ ] = 1%r.
+proof. by conseq state_init_ref_ll (state_init_ref_h _r8). qed.
+
+
+lemma addratebit_ref_ll: islossless M.__addratebit_ref
+ by islossless.
+
+hoare addratebit_ref_h _r8 _st:
+ M.__addratebit_ref
+ : st = _st /\ rATE8=_r8
+ ==> res = addratebit _r8 _st.
+proof.
+admit (* BDEP? *).
+qed.
+
+phoare addratebit_ref_ph _r8 _st:
+ [ M.__addratebit_ref
+ : st = _st /\ rATE8=_r8
+ ==> res = addratebit _r8 _st
+ ] = 1%r.
+proof. by conseq addratebit_ref_ll (addratebit_ref_h _r8 _st). qed.
 
